restructured Slicing

thys/Slicing/Dynamic/DynPDG.thy
@@ -1,6 +1,12 @@
-header {* \isaheader{PDG} *}
+header {*  \isachapter{Dynamic Slicing} 
+  \isaheader{Dynamic Program Dependence Graph} *}
 
-theory PDG imports DataDependence CFGExit_wf begin
+theory DynPDG imports 
+  "../Basic/DynDataDependence" 
+  "../Basic/CFGExit_wf" 
+  "../Basic/DynStandardControlDependence"
+  "../Basic/DynWeakControlDependence"
+begin
 
 subsection {* The dynamic PDG *}
 
@@ -378,153 +384,89 @@ qed
 end
 
 
-subsection {* The static PDG *}
+subsection {* Instantiate dynamic PDG *}
 
-locale PDG = 
+subsubsection {* Standard control dependence *}
+
+locale DynStandardControlDependencePDG =
+  Postdomination sourcenode targetnode kind valid_edge Entry Exit +
   CFGExit_wf sourcenode targetnode kind valid_edge Entry Def Use state_val Exit
   for sourcenode :: "'edge \<Rightarrow> 'node" and targetnode :: "'edge \<Rightarrow> 'node"
   and kind :: "'edge \<Rightarrow> 'state edge_kind" and valid_edge :: "'edge \<Rightarrow> bool"
   and Entry :: "'node" ("'('_Entry'_')") and Def :: "'node \<Rightarrow> 'var set"
   and Use :: "'node \<Rightarrow> 'var set" and state_val :: "'state \<Rightarrow> 'var \<Rightarrow> 'val"
-  and Exit :: "'node" ("'('_Exit'_')") +
-  fixes control_dependence :: "'node \<Rightarrow> 'node \<Rightarrow> bool" 
-("_ controls _ " [51,0])
-  assumes Exit_not_control_dependent:"n controls n' \<Longrightarrow> n' \<noteq> (_Exit_)"
-  assumes control_dependence_path:
-  "n controls n' 
-  \<Longrightarrow> \<exists>as. CFG.path sourcenode targetnode valid_edge n as n' \<and> as \<noteq> []"
+  and Exit :: "'node" ("'('_Exit'_')")
 
 begin
 
-
-inductive cdep_edge :: "'node \<Rightarrow> 'node \<Rightarrow> bool" 
-    ("_ \<longrightarrow>\<^bsub>cd\<^esub> _" [51,0] 80)
-  and ddep_edge :: "'node \<Rightarrow> 'var \<Rightarrow> 'node \<Rightarrow> bool"
-    ("_ -_\<rightarrow>\<^bsub>dd\<^esub> _" [51,0,0] 80)
-  and PDG_edge :: "'node \<Rightarrow> 'var option \<Rightarrow> 'node \<Rightarrow> bool"
-
-where
-    (* Syntax *)
-  "n \<longrightarrow>\<^bsub>cd\<^esub> n' == PDG_edge n None n'"
-  | "n -V\<rightarrow>\<^bsub>dd\<^esub> n' == PDG_edge n (Some V) n'"
-
-    (* Rules *)
-  | PDG_cdep_edge:
-  "n controls n' \<Longrightarrow> n \<longrightarrow>\<^bsub>cd\<^esub> n'"
-
-  | PDG_ddep_edge:
-  "n influences V in n' \<Longrightarrow> n -V\<rightarrow>\<^bsub>dd\<^esub> n'"
-
-
-inductive PDG_path :: "'node \<Rightarrow> 'node \<Rightarrow> bool"
-("_ \<longrightarrow>\<^isub>d* _" [51,0] 80) 
-
-where PDG_path_Nil:
-  "valid_node n \<Longrightarrow> n \<longrightarrow>\<^isub>d* n"
-
-  | PDG_path_Append_cdep:
-  "\<lbrakk>n \<longrightarrow>\<^isub>d* n''; n'' \<longrightarrow>\<^bsub>cd\<^esub> n'\<rbrakk> \<Longrightarrow> n \<longrightarrow>\<^isub>d* n'"
-
-  | PDG_path_Append_ddep:
-  "\<lbrakk>n \<longrightarrow>\<^isub>d* n''; n'' -V\<rightarrow>\<^bsub>dd\<^esub> n'\<rbrakk> \<Longrightarrow> n \<longrightarrow>\<^isub>d* n'"
-
-
-lemma PDG_path_cdep:"n \<longrightarrow>\<^bsub>cd\<^esub> n' \<Longrightarrow> n \<longrightarrow>\<^isub>d* n'"
-apply -
-apply(rule PDG_path_Append_cdep, rule PDG_path_Nil)
-by(auto elim!:PDG_edge.cases dest:control_dependence_path path_valid_node)
-
-lemma PDG_path_ddep:"n -V\<rightarrow>\<^bsub>dd\<^esub> n' \<Longrightarrow> n \<longrightarrow>\<^isub>d* n'"
-apply -
-apply(rule PDG_path_Append_ddep, rule PDG_path_Nil)
-by(auto elim!:PDG_edge.cases dest:path_valid_node simp:data_dependence_def)
-
-lemma PDG_path_Append:
-  "\<lbrakk>n'' \<longrightarrow>\<^isub>d* n'; n \<longrightarrow>\<^isub>d* n''\<rbrakk> \<Longrightarrow> n \<longrightarrow>\<^isub>d* n'"
-by(induct rule:PDG_path.induct,auto intro:PDG_path.intros)
-
-
-lemma PDG_cdep_edge_CFG_path:
-  assumes "n \<longrightarrow>\<^bsub>cd\<^esub> n'" obtains as where "n -as\<rightarrow>* n'" and "as \<noteq> []"
-  using `n \<longrightarrow>\<^bsub>cd\<^esub> n'`
-  by(auto elim:PDG_edge.cases dest:control_dependence_path)
-
-lemma PDG_ddep_edge_CFG_path:
-  assumes "n -V\<rightarrow>\<^bsub>dd\<^esub> n'" obtains as where "n -as\<rightarrow>* n'" and "as \<noteq> []"
-  using `n -V\<rightarrow>\<^bsub>dd\<^esub> n'`
-  by(auto elim!:PDG_edge.cases simp:data_dependence_def)
-
-lemma PDG_path_CFG_path:
-  assumes "n \<longrightarrow>\<^isub>d* n'" obtains as where "n -as\<rightarrow>* n'"
-proof(atomize_elim)
-  from `n \<longrightarrow>\<^isub>d* n'` show "\<exists>as. n -as\<rightarrow>* n'"
-  proof(induct rule:PDG_path.induct)
-    case (PDG_path_Nil n)
-    hence "n -[]\<rightarrow>* n" by(rule empty_path)
-    thus ?case by blast
-  next
-    case (PDG_path_Append_cdep n n'' n')
-    from `n'' \<longrightarrow>\<^bsub>cd\<^esub> n'` obtain as where "n'' -as\<rightarrow>* n'"
-      by(fastsimp elim:PDG_cdep_edge_CFG_path)
-    with `\<exists>as. n -as\<rightarrow>* n''` obtain as' where "n -as'@as\<rightarrow>* n'"
-      by(auto dest:path_Append)
-    thus ?case by blast
-  next
-    case (PDG_path_Append_ddep n n'' V n')
-    from `n'' -V\<rightarrow>\<^bsub>dd\<^esub> n'` obtain as where "n'' -as\<rightarrow>* n'"
-      by(fastsimp elim:PDG_ddep_edge_CFG_path)
-    with `\<exists>as. n -as\<rightarrow>* n''` obtain as' where "n -as'@as\<rightarrow>* n'"
-      by(auto dest:path_Append)
-    thus ?case by blast
+lemma DynPDG_scd:
+  "DynPDG sourcenode targetnode kind valid_edge (_Entry_) 
+          Def Use state_val (_Exit_) dyn_standard_control_dependence"
+proof(unfold_locales)
+  fix n n' as assume "n controls\<^isub>s n' via as"
+  show "n' \<noteq> (_Exit_)"
+  proof
+    assume "n' = (_Exit_)"
+    with `n controls\<^isub>s n' via as` show False
+      by(fastsimp intro:Exit_not_dyn_standard_control_dependent)
   qed
-qed
-
-
-lemma PDG_path_Exit:"\<lbrakk>n \<longrightarrow>\<^isub>d* n'; n' = (_Exit_)\<rbrakk> \<Longrightarrow> n = (_Exit_)"
-apply(induct rule:PDG_path.induct)
-by(auto elim:PDG_edge.cases dest:Exit_not_control_dependent 
-        simp:data_dependence_def)
-
-
-lemma PDG_path_not_inner:
-  "\<lbrakk>n \<longrightarrow>\<^isub>d* n'; \<not> inner_node n'\<rbrakk> \<Longrightarrow> n = n'"
-proof(induct rule:PDG_path.induct)
-  case (PDG_path_Nil n)
-  thus ?case by simp
 next
-  case (PDG_path_Append_cdep n n'' n')
-  from `n'' \<longrightarrow>\<^bsub>cd\<^esub> n'` `\<not> inner_node n'` have False
-    apply -
-    apply(erule PDG_edge.cases) apply(auto simp:inner_node_def)
-      apply(fastsimp dest:control_dependence_path path_valid_node)
-     apply(fastsimp dest:control_dependence_path path_valid_node)
-    by(fastsimp dest:Exit_not_control_dependent)
-  thus ?case by simp
-next
-  case (PDG_path_Append_ddep n n'' V n')
-  from `n'' -V\<rightarrow>\<^bsub>dd\<^esub> n'` `\<not> inner_node n'` have False
-    apply -
-    apply(erule PDG_edge.cases) 
-    by(auto dest:path_valid_node simp:inner_node_def data_dependence_def)
-  thus ?case by simp
+  fix n n' as assume "n controls\<^isub>s n' via as"
+  thus "n -as\<rightarrow>* n' \<and> as \<noteq> []"
+    by(fastsimp simp:dyn_standard_control_dependence_def)
 qed
-
-
-subsubsection {* Definition of the static backward slice *}
-
-definition PDG_BS :: "'node \<Rightarrow> 'node set"
-  where "PDG_BS n \<equiv> (if valid_node n then {n'. n' \<longrightarrow>\<^isub>d* n} else {})"
-
-
-lemma PDG_BS_valid_node:"n \<in> PDG_BS n\<^isub>c \<Longrightarrow> valid_node n"
-  by(auto elim:PDG_path_CFG_path dest:path_valid_node simp:PDG_BS_def 
-          split:split_if_asm)
-
-lemma Exit_PDG_BS:"n \<in> PDG_BS (_Exit_) \<Longrightarrow> n = (_Exit_)"
-  by(fastsimp dest:PDG_path_Exit simp:PDG_BS_def)
 
 
 end
 
+subsubsection {* Weak control dependence *}
+
+locale DynWeakControlDependencePDG = 
+  StrongPostdomination sourcenode targetnode kind valid_edge Entry Exit +
+  CFGExit_wf sourcenode targetnode kind valid_edge Entry Def Use state_val Exit
+  for sourcenode :: "'edge \<Rightarrow> 'node" and targetnode :: "'edge \<Rightarrow> 'node"
+  and kind :: "'edge \<Rightarrow> 'state edge_kind" and valid_edge :: "'edge \<Rightarrow> bool"
+  and Entry :: "'node" ("'('_Entry'_')") and Def :: "'node \<Rightarrow> 'var set"
+  and Use :: "'node \<Rightarrow> 'var set" and state_val :: "'state \<Rightarrow> 'var \<Rightarrow> 'val"
+  and Exit :: "'node" ("'('_Exit'_')")
+
+begin
+
+lemma DynPDG_wcd:
+  "DynPDG sourcenode targetnode kind valid_edge (_Entry_) 
+          Def Use state_val (_Exit_) dyn_weak_control_dependence"
+proof(unfold_locales)
+  fix n n' as assume "n weakly controls n' via as"
+  show "n' \<noteq> (_Exit_)"
+  proof
+    assume "n' = (_Exit_)"
+    with `n weakly controls n' via as` show False
+      by(fastsimp intro:Exit_not_dyn_weak_control_dependent)
+  qed
+next
+  fix n n' as assume "n weakly controls n' via as"
+  thus "n -as\<rightarrow>* n' \<and> as \<noteq> []"
+    by(fastsimp simp:dyn_weak_control_dependence_def)
+qed
+
+
 end
 
+
+subsection {* Data slice *}
+
+definition (in CFG) empty_control_dependence :: "'node \<Rightarrow> 'node \<Rightarrow> 'edge list \<Rightarrow> bool"
+where "empty_control_dependence n n' as \<equiv> False"
+
+lemma (in CFGExit_wf) DynPDG_scd:
+  "DynPDG sourcenode targetnode kind valid_edge (_Entry_)
+          Def Use state_val  (_Exit_) empty_control_dependence"
+proof(unfold_locales)
+  fix n n' as assume "empty_control_dependence n n' as"
+  thus "n' \<noteq> (_Exit_)" by(simp add:empty_control_dependence_def)
+next
+  fix n n' as assume "empty_control_dependence n n' as"
+  thus "n -as\<rightarrow>* n' \<and> as \<noteq> []" by(simp add:empty_control_dependence_def)
+qed
+
+end
