thys/Slicing/StaticIntra/StandardControlDependence.thy
@@ -1,0 +1,47 @@
+header {* \isaheader{Static Standard Control Dependence} *}
+
+theory StandardControlDependence imports 
+  "../Basic/Postdomination" 
+  "../Basic/DynStandardControlDependence"
+begin
+
+context Postdomination begin
+
+subsubsection {* Definition and some lemmas *}
+
+definition standard_control_dependence :: "'node \<Rightarrow> 'node \<Rightarrow> bool" 
+  ("_ controls\<^isub>s _" [51,0])
+where standard_control_dependences_eq:"n controls\<^isub>s n' \<equiv> \<exists>as. n controls\<^isub>s n' via as"
+
+lemma standard_control_dependence_def:"n controls\<^isub>s n' =
+    (\<exists>a a' as. (n' \<notin> set(sourcenodes (a#as))) \<and> (n -a#as\<rightarrow>* n') \<and>
+                   (n' postdominates (targetnode a)) \<and>
+                   (valid_edge a') \<and> (sourcenode a' = n) \<and> 
+                   (\<not> n' postdominates (targetnode a')))"
+by(auto simp:standard_control_dependences_eq dyn_standard_control_dependence_def)
+
+
+lemma Exit_not_standard_control_dependent:
+  "n controls\<^isub>s (_Exit_) \<Longrightarrow> False"
+by(auto simp:standard_control_dependences_eq 
+        intro:Exit_not_dyn_standard_control_dependent)
+             
+
+lemma standard_control_dependence_def_variant:
+  "n controls\<^isub>s n' = (\<exists>as. (n -as\<rightarrow>* n') \<and> (n \<noteq> n') \<and>
+    (\<not> n' postdominates n) \<and> (n' \<notin> set(sourcenodes as)) \<and>
+  (\<forall>n'' \<in> set(targetnodes as). n' postdominates n''))"
+by(auto simp:standard_control_dependences_eq 
+             dyn_standard_control_dependence_def_variant)
+
+
+lemma inner_node_standard_control_dependence_predecessor:
+  assumes "inner_node n" "(_Entry_) -as\<rightarrow>* n" "n -as'\<rightarrow>* (_Exit_)"
+  obtains n' where "n' controls\<^isub>s n"
+using assms
+by(auto elim!:inner_node_dyn_standard_control_dependence_predecessor
+        simp:standard_control_dependences_eq)
+
+end
+
+end
